

Homework of Optimal Estimation

Junda Wu 255065010

Homework 1

1. Proof Since X and Y are uncorrelated, we have $\text{Cov}(X, Y) = E[(X - EX)(Y - EY)] = 0$. Hence

$$C_Z = \begin{bmatrix} \sigma_x^2 & 0 \\ 0 & \sigma_y^2 \end{bmatrix}$$

Then $|\det C_Z|^{1/2} = \sigma_x \sigma_y$, $C_Z^{-1} = \begin{bmatrix} 1/\sigma_x^2 & 0 \\ 0 & 1/\sigma_y^2 \end{bmatrix}$

Since X, Y are jointly normal, we have

$$f(x, y) = \frac{1}{2\pi\sigma_x\sigma_y} \exp \left[-\frac{(x-EX)^2}{2\sigma_x^2} - \frac{(y-EY)^2}{2\sigma_y^2} \right]$$

Then we can calculate marginal distribution:

$$\begin{aligned} f_X(x) &= \int_{-\infty}^{+\infty} f(x, y) dy = \frac{1}{\sqrt{2\pi}\sigma_x} \exp \left[-\frac{(x-EX)^2}{2\sigma_x^2} \right] \frac{1}{\sqrt{2\pi}\sigma_y} \int_{-\infty}^{+\infty} \exp \left[-\frac{(y-EY)^2}{2\sigma_y^2} \right] dy \\ &= \frac{1}{\sqrt{2\pi}\sigma_x} \exp \left[-\frac{(x-EX)^2}{2\sigma_x^2} \right] \underbrace{\frac{1}{\sqrt{2\pi}\sigma} \int_{-\infty}^{+\infty} \exp \left[-\frac{(x-\mu)^2}{2\sigma^2} \right] dx}_{\text{recall that}} = 1 \end{aligned}$$

Similarly, $f_Y(y) = \frac{1}{\sqrt{2\pi}\sigma_y} \exp \left[-\frac{(y-EY)^2}{2\sigma_y^2} \right]$

Note that $f(x, y) = f_X(x)f_Y(y)$, we can conclude that X and Y are independent. □

2. Solution

$$\begin{aligned} (1) \quad R_Z(i, j) &= E(z(i)z(j)) = E(s^2 + s(v(i) + v(j)) + v(i)v(j)) \\ &= E(s^2) + E(sv(i)) + E(sv(j)) + E(v(i)v(j)) = \begin{cases} 5, & i=j \\ 4, & i \neq j \end{cases} \\ &\quad \begin{matrix} = 2 & = 1 & = 1 & = \end{matrix} \begin{cases} 0, & i \neq j \\ \text{Var}(v(i)) = 1, & i=j \end{cases} \end{aligned}$$

(2) $E(z(n)) = E(s) + E(v(n)) = 1 \Rightarrow E(z(n))$ is constant

$\Rightarrow z(n)$ is WSS. □

$R_Z(k) = \begin{cases} 4, & k \neq 0 \\ 5, & k = 0 \end{cases} \Rightarrow R_Z(k)$ is independent of time

Homework 2

1. Solution Maximum Likelihood:

$$P(Y = \{b, 2, 6\} | X = \{1, 1, 1\}) = \overset{\frac{1}{6}}{P(Y=b|X=1)} \overset{\frac{1}{6}}{P(Y=2|X=1)} \overset{\frac{1}{6}}{P(Y=6|X=1)} = \frac{1}{216}$$

$$P(Y = \{b, 2, 6\} | X = \{1, 0, 1\}) = \frac{1}{6} \times \frac{1}{10} \times \frac{1}{6} = \frac{1}{360}$$

$$P(Y = \{b, 2, 6\} | X = \{0, 1, 1\}) = \frac{1}{2} \times \frac{1}{6} \times \frac{1}{6} = \frac{1}{72}$$

$$P(Y = \{b, 2, 6\} | X = \{1, 1, 0\}) = \frac{1}{6} \times \frac{1}{6} \times \frac{1}{2} = \frac{1}{72}$$

$$P(Y = \{b, 2, 6\} | X = \{1, 0, 0\}) = \frac{1}{6} \times \frac{1}{10} \times \frac{1}{2} = \frac{1}{120} \Rightarrow X_{ML} = \{0, 1, 0\}$$

$$P(Y = \{b, 2, 6\} | X = \{0, 0, 1\}) = \frac{1}{2} \times \frac{1}{10} \times \frac{1}{6} = \frac{1}{120}$$

$$P(Y = \{b, 2, 6\} | X = \{0, 1, 0\}) = \frac{1}{2} \times \frac{1}{6} \times \frac{1}{2} = \frac{1}{24}$$

$$P(Y = \{b, 2, 6\} | X = \{0, 0, 0\}) = \frac{1}{2} \times \frac{1}{10} \times \frac{1}{2} = \frac{1}{40}$$

$$MAP: \lim_{n \rightarrow \infty} A^n = \begin{bmatrix} \frac{2}{3} & \frac{1}{3} \\ \frac{2}{3} & \frac{1}{3} \end{bmatrix} \Rightarrow P(X=0) = \frac{1}{3} \quad P(X=1) = \frac{2}{3}$$

$$P(X|Y) = \frac{P(Y|X)P(X)}{P(Y)} \propto P(Y|X)P(X)$$

So we can compute

$$P(X = \{1, 1, 1\}) P(Y = \{b, 2, 6\} | X = \{1, 1, 1\}) = \frac{1}{216} \times \frac{2}{3} \times 0.95 \times 0.95 = \frac{361}{129600}$$

$$P(X = \{1, 0, 1\}) P(Y = \{b, 2, 6\} | X = \{1, 0, 1\}) = \frac{1}{360} \times \frac{2}{3} \times 0.05 \times 0.1 = \frac{1}{108000}$$

$$P(X = \{0, 1, 1\}) P(Y = \{b, 2, 6\} | X = \{0, 1, 1\}) = \frac{1}{72} \times \frac{1}{3} \times 0.1 \times 0.95 = \frac{19}{43200} = \frac{57}{129600}$$

$$P(X = \{1, 1, 0\}) P(Y = \{b, 2, 6\} | X = \{1, 1, 0\}) = \frac{1}{72} \times \frac{2}{3} \times 0.95 \times 0.05 = \frac{19}{43200}$$

$$P(X = \{1, 0, 0\}) P(Y = \{b, 2, 6\} | X = \{1, 0, 0\}) = \frac{1}{120} \times \frac{2}{3} \times 0.05 \times 0.1 = \frac{1}{36000} = \frac{1}{4000}$$

$$P(X = \{0, 0, 1\}) P(Y = \{b, 2, 6\} | X = \{0, 0, 1\}) = \frac{1}{120} \times \frac{1}{3} \times 0.1 \times 0.1 = \frac{1}{4000}$$

$$\text{So, } X_{MAP} = \{0, 0, 0\}.$$

$$P(X = \{0, 1, 0\}) P(Y = \{b, 2, 6\} | X = \{0, 1, 0\}) = \frac{1}{24} \times \frac{1}{3} \times 0.1 \times 0.05 = \frac{1}{14400}$$

$$P(X = \{0, 0, 0\}) P(Y = \{b, 2, 6\} | X = \{0, 0, 0\}) = \frac{1}{40} \times \frac{1}{3} \times 0.9 \times 0.9 = \frac{81}{12000} = \frac{27}{4000} \rightarrow \text{maximum}$$

2. Solution

$$(1) \quad (a) \quad f(z|s) = f_V(V)|_{V=z-s} = \frac{1}{\sqrt{2\pi}V} e^{-\frac{(z-s)^2}{2V^2}}$$

$$f_S(s) = \frac{1}{\sqrt{2\pi}\sigma} \exp\left[-\frac{(s-\eta)^2}{2\sigma^2}\right] \quad f_Z(z) = \frac{1}{\sqrt{2\pi}\sqrt{\sigma^2+V^2}} \exp\left[-\frac{(z-\eta)^2}{2(\sigma^2+V^2)}\right]$$

$$\Rightarrow f_S(s|z=z) = \frac{f_Z(z|s)f_S(s)}{f_Z(z)}$$

$$= \frac{1}{2\pi\sigma V \frac{1}{\sqrt{2\pi}\sqrt{\sigma^2+V^2}}} \exp\left\{-\frac{(z-s)^2}{2V^2} - \frac{(s-\eta)^2}{2\sigma^2} + \frac{(z-\eta)^2}{2(\sigma^2+V^2)}\right\}$$

$$= \frac{1}{\sqrt{2\pi} \sqrt{\frac{\sigma^2 V^2}{\sigma^2+V^2}}} \exp \frac{-\sigma^2(\sigma^2+V^2)(\cancel{z^2}-2\cancel{z}s+\cancel{s^2}) - V^2(\sigma^2+V^2)(\cancel{s^2}-\cancel{2s\eta}+\cancel{\eta^2}) + \sigma^2 V^2(\cancel{z^2}-\cancel{2\eta z}+\cancel{\eta^2})}{2(V^2)(\sigma^2)(\sigma^2+V^2)}$$

$$= \frac{1}{\sqrt{2\pi} \sqrt{\frac{\sigma^2 V^2}{\sigma^2+V^2}}} \exp \frac{1}{2V^2\sigma^2(\sigma^2+V^2)} \left\{ -(\sigma^2+V^2)^2 s^2 + s \left(\sigma^2(\sigma^2+V^2)2z + V^2(\sigma^2+V^2)2\eta \right) - \left[\sigma^4 z^2 + V^4 \eta^2 + 2\eta z \sigma^2 V^2 \right] \right\}$$

$(\sigma^2 z + V^2 \eta)^2$

$$= \frac{1}{\sqrt{2\pi} \sqrt{\frac{\sigma^2 V^2}{\sigma^2+V^2}}} \exp \left[-\frac{\left[(\sigma^2+V^2)s - (\sigma^2 z + V^2 \eta) \right]^2}{2V^2\sigma^2(\sigma^2+V^2)} \right]$$

$$= \frac{1}{\sqrt{2\pi} \sqrt{\frac{\sigma^2 V^2}{\sigma^2+V^2}}} \exp \left[-\frac{1}{2 \frac{V^2 \sigma^2}{\sigma^2+V^2}} \left[s - \left(\frac{\sigma^2}{\sigma^2+V^2} z + \frac{V^2}{\sigma^2+V^2} \eta \right) \right]^2 \right]$$

$$\Rightarrow E[s|z=z] = \frac{\sigma^2}{\sigma^2+V^2} z + \frac{V^2}{\sigma^2+V^2} \eta = \eta + \frac{\sigma^2}{\sigma^2+V^2} (z-\eta)$$

$$(b) \quad E[s^2|z=z] = D[s|z=z] + E[s|z=z]^2 = \frac{\sigma^2 V^2}{\sigma^2+V^2} + \left(\eta + \frac{\sigma^2}{\sigma^2+V^2} (z-\eta) \right)^2$$

(2) (a) Maximum Likelihood Estimate.

$$f_Z(z=z(i)|s) = \frac{1}{\sqrt{2\pi}\sigma_V} \exp\left[-\frac{(z(i)-s)^2}{2\sigma_V^2}\right]$$

So we have the likelihood function

$$f_Z(z=z(1), \dots, z(n)|s) = \prod_{i=1}^n \frac{1}{\sqrt{2\pi}\sigma_V} \exp\left[-\frac{(z(i)-s)^2}{2\sigma_V^2}\right]$$

To maximize the above function, consider logarithm of it:

$$\ln f_Z = -n \ln(\sqrt{2\pi} \sigma_V) - \sum_{i=1}^n \frac{(z(i)-s)^2}{2\sigma_V^2} \Rightarrow \frac{\partial f_Z}{\partial s} = \frac{n}{\sum_{i=1}^n} \frac{z(i)-s}{\sigma_V^2} = 0 \Rightarrow \hat{S}_{ML} = \frac{1}{n} \sum_{i=1}^n z(i)$$

(b) Maximum A Posteriori estimate (MAP):

$$\begin{aligned} f_S(s|z=z(1), \dots, z(n)) &\propto f_S(s) f_Z(z=z(1), \dots, z(n)|s) \\ &= \underbrace{\frac{1}{\prod_{i=1}^n \sqrt{2\pi} \sigma_V} \exp\left[-\frac{(z(i)-s)^2}{2\sigma_V^2}\right]}_{\text{likelihood}} \times \underbrace{\frac{1}{\sqrt{2\pi} \sigma_S} \exp\left[-\frac{(s-\eta_S)^2}{2\sigma_S^2}\right]}_{\text{prior}} \end{aligned}$$

Again, consider the logarithm to maximize it:

$$\ln f_Z = -n \ln(\sqrt{2\pi} \sigma_V) - \ln(\sqrt{2\pi} \sigma_S) - \sum_{i=1}^n \frac{(z(i)-s)^2}{2\sigma_V^2} - \frac{(s-\eta_S)^2}{2\sigma_S^2}$$

$$\begin{aligned} \frac{\partial \ln f_Z}{\partial s} &= \sum_{i=1}^n \frac{(z(i)-s)}{\sigma_V^2} - \frac{s-\eta_S}{\sigma_S^2} = 0 \Rightarrow \hat{S}_{MAP} = \frac{\sigma_S^2}{n\sigma_S^2 + \sigma_V^2} \sum_{i=1}^n z(i) + \frac{\sigma_V^2}{n\sigma_S^2 + \sigma_V^2} \eta_S \\ &\Downarrow \\ -\frac{n}{\sigma_V^2} s + \frac{1}{\sigma_V^2} \sum_{i=1}^n z(i) - \frac{s}{\sigma_S^2} + \frac{\eta_S}{\sigma_S^2} &= 0 \Rightarrow -n\sigma_S^2 s + \sigma_S^2 \sum_{i=1}^n z(i) - \sigma_V^2 s + \sigma_V^2 \eta_S = 0 \end{aligned}$$

$$(c) f(s=s, z_1=z(1), \dots, z_n=z(n)) = f(s=s, v_1=z(1)-s, \dots, v_n=z(n)-s)$$

Since s and v are independent, define $\vec{v} = [v_1, \dots, v_n]$, we have $\begin{bmatrix} s \\ \vec{v} \end{bmatrix} \sim N\left(\begin{bmatrix} \eta_S \\ 0 \end{bmatrix}, \begin{bmatrix} \sigma_S^2 & \\ & \sigma_V^2 I \end{bmatrix}\right)$

$$\begin{aligned} \text{Hence } f(s=s, v_1=z(1)-s, \dots, v_n=z(n)-s) &= \frac{1}{\sigma_S^2} (s-\eta_S)^2 + \frac{1}{\sigma_V^2} \sum_{i=1}^n (z_i-s)^2 = \frac{1}{\sigma_S^2} (s-\eta_S)^2 + \frac{1}{\sigma_V^2} \sum_{i=1}^n (z_i^2 + s^2 - 2sz_i) \\ &= \frac{1}{(2\pi)^{\frac{n+1}{2}} \sigma_S \sigma_V^n} \exp\left(-\frac{1}{2} \begin{bmatrix} (s-\eta_S) & (\vec{z}-s\vec{1})^T \end{bmatrix} \begin{bmatrix} \sigma_S^2 & \\ & \sigma_V^2 I \end{bmatrix}^{-1} \begin{bmatrix} s-\eta_S \\ \vec{z}-s\vec{1} \end{bmatrix}\right) \end{aligned}$$

On the other hand, $\vec{z} \sim N(\eta_S \vec{1}, (\sigma_S^2 + \sigma_V^2) I)$. Therefore, $\frac{1}{\sigma_V^2 + \sigma_S^2} \sum_{i=1}^n (z_i^2 - 2\eta_S z_i + \eta_S^2)$

$$f(z=z(1), \dots, z(n)) = \frac{1}{(2\pi)^{\frac{n}{2}} (\sigma_S + \sigma_V)^n} \exp\left(-\frac{1}{2} \begin{bmatrix} \vec{z} - \eta_S \vec{1} \end{bmatrix}^T \begin{bmatrix} (\sigma_V^2 + \sigma_S^2) I \end{bmatrix}^{-1} \begin{bmatrix} \vec{z} - \eta_S \vec{1} \end{bmatrix}\right)$$

$$\begin{aligned} \text{Then, by Bayes equation, } f(s|z_1=z(1), \dots, z_n=z(n)) &= \frac{f(s=s, z_1=z(1), \dots, z_n=z(n))}{f(z_1=z(1), \dots, z_n=z(n))} \\ &= \frac{(\sigma_S + \sigma_V)^n}{\sqrt{2\pi} \sigma_S \sigma_V^n} \exp\left[\left(\frac{1}{\sigma_S^2} + \frac{n}{\sigma_V^2}\right) s^2 - \frac{2\eta_S}{\sigma_S^2} s - \frac{2}{\sigma_V^2} \sum_{i=1}^n z(i) s + \dots\right] \end{aligned}$$

Note that it's a Gaussian distribution, thus

$$\hat{S}_{MMSE} = E(s|z_1=z(1), \dots, z_n=z(n)) = \frac{1}{\frac{1}{\sigma_S^2} + \frac{n}{\sigma_V^2}} \left(\frac{\eta_S}{\sigma_S^2} + \frac{1}{\sigma_V^2} \sum_{i=1}^n z(i) \right) = \frac{1}{\sigma_V^2 + n\sigma_S^2} \left(\eta_S \sigma_V^2 + \sigma_S^2 \sum_{i=1}^n z(i) \right)$$

Note that in this case, $\hat{S}_{MAP} = \hat{S}_{MMSE}$!

$$(d) \quad E[z(i)] = E[s + v(i)] = E[s] + E[v(i)] = \text{Var}(s) + E[s] = \eta_s^2 + \sigma_s^2$$

$$E[z(i)z(j)] = E[s^2] + E[s]E[v(i)+v(j)] + E[v(i)v(j)] = \begin{cases} \sigma_s^2 + \eta_s^2 & i=j \\ \sigma_s^2 + \eta_s^2 + \sigma_v^2 & i \neq j \end{cases}$$

$$E[zz^T] = \sigma_v^2 I + (\eta_s^2 + \sigma_s^2) M \quad M = \begin{bmatrix} 1 & \dots & 1 \\ \vdots & & \vdots \\ 1 & \dots & 1 \end{bmatrix}$$

$$= \sigma_v^2 I + (\eta_s^2 + \sigma_s^2) \begin{bmatrix} 1 \\ \vdots \\ 1 \end{bmatrix} \begin{bmatrix} 1 & \dots & 1 \end{bmatrix}$$

Lemma. For $A = kI + lxx^T$, we have its inverse as $A^{-1} = \frac{1}{k}I - \frac{l}{k(k+lx^Tx)}xx^T$

Proof of Lemma.

$$AA^{-1} = (kI + lxx^T) \left(\frac{1}{k}I - \frac{l}{k(k+lx^Tx)}xx^T \right)$$

$$= I - \frac{l^2 x^T x}{k(k+lx^Tx)}xx^T + \frac{l}{k}xx^T - \frac{kl}{k(k+lx^Tx)}xx^T$$

$$= I + \frac{-l^2 x^T x + l(k+lx^Tx) - kl}{k(k+lx^Tx)}xx^T = I \quad \square$$

$$x^T x = n, \quad k = \sigma_v^2, \quad l = \sigma_s^2 + \eta_s^2$$

$$\Rightarrow E^{-1}(zz^T) = \frac{1}{\sigma_v^2}I - \frac{(\eta_s^2 + \sigma_s^2)}{\sigma_v^2[\sigma_v^2 + (\eta_s^2 + \sigma_s^2)n]} M = \frac{1}{\sigma_v^2[\sigma_v^2 + (\eta_s^2 + \sigma_s^2)n]} \begin{bmatrix} \sigma_v^2 + (n-1)(\sigma_s^2 + \eta_s^2) & \dots & -(\sigma_s^2 + \eta_s^2) \\ \vdots & & \vdots \\ -(\sigma_s^2 + \eta_s^2) & \dots & \sigma_v^2 + (n-1)(\sigma_s^2 + \eta_s^2) \end{bmatrix}$$

$$E[sz^T] [E(zz^T)]^{-1} = \frac{\eta_s^2 + \sigma_s^2}{\sigma_v^2[\sigma_v^2 + (\eta_s^2 + \sigma_s^2)n]} [\sigma_v^2, \dots, \sigma_v^2] = \frac{\eta_s^2 + \sigma_s^2}{[\sigma_v^2 + (\eta_s^2 + \sigma_s^2)n]} \mathbf{1}$$

$$\Rightarrow \hat{S}_{LMMSE} = E[sz^T] [E(zz^T)]^{-1} [z(1), \dots, z(n)]^T = \frac{\eta_s^2 + \sigma_s^2}{\sigma_v^2 + (\eta_s^2 + \sigma_s^2)n} \sum_{i=1}^n z(i)$$

(e) Since $\begin{bmatrix} z(1) \\ \vdots \\ z(n) \end{bmatrix} = \begin{bmatrix} 1 \\ \vdots \\ 1 \end{bmatrix} s + v$, $\hat{S}_{LS} = (H^T H)^{-1} H^T \begin{bmatrix} z(1) \\ \vdots \\ z(n) \end{bmatrix} = \frac{1}{n} \sum_{i=1}^n z(i)$

Note that $\hat{S}_{LS} = \hat{S}_{ML}$!

(f) $z_k = s + v_k$, $\hat{S}_0 = E[s] = \eta_s$, $H_k = 1$, $R_k = \sigma_v^2$, $P_0 = \sigma_s^2$

Iteration:

$$\begin{cases} K_k = P_{k-1} H_k^T (H_k P_{k-1} H_k^T + R_k)^{-1} = P_{k-1} (P_{k-1} + R_k)^{-1} \\ P_k = [I - K_k H_k] P_{k-1} = (1 - K_k) P_{k-1} \\ \hat{S}_k = \hat{S}_{k-1} + K_k (z_k - H_k \hat{S}_{k-1}) = (1 - K_k) \hat{S}_{k-1} + K_k z_k \end{cases}$$

By iteration, we obtain

$$\begin{cases} k = \frac{\sigma_s^2}{k\sigma_s^2 + \sigma_v^2} \\ \hat{s}_k = \frac{\sigma_s^2 \sum_{i=1}^k z(i) + \sigma_v^2 \eta_s}{k\sigma_s^2 + \sigma_v^2} \\ p_k = \frac{\sigma_s^2 \sigma_v^2}{k\sigma_s^2 + \sigma_v^2} \end{cases}$$

$$\Rightarrow \hat{s}_{RLS} = \hat{s}_N = \frac{\sigma_s^2 \sum_{i=1}^n z(i) + \sigma_v^2 \eta_s}{n\sigma_s^2 + \sigma_v^2}$$

Note that $\hat{s}_{RLS} = \hat{s}_{MAP} = \hat{s}_{MMSE}$!

(g) ① Maximum Likelihood Estimate:

It maximizes the likelihood function based on data only without prior knowledge.

Advantage: Simple, easy to compute.

Disadvantage: Lacks consideration of prior information, sensitive to noise

② Maximum A Posteriori (MAP) Estimate:

Combines likelihood and prior distribution.

Advantage: Utilizes prior knowledge

Disadvantage: Depends on the choice of prior distribution.

③ Minimum Mean Square Estimate (MMSE):

Minimizes mean square error using posteriori distribution.

Advantage: Optimal for mean squared error.

Disadvantage: Computationally complex.

④ Linear Minimum Mean Square Estimate (LMMSE)

A linear form of MMSE.

Advantage: Easier to compute.

Disadvantage: It's biased, may be less accurate for nonlinear relations.

⑤ Least Squares Estimate:

Minimizes sum of squared errors.

Advantage: Easy to understand and implement, low computational cost.

Disadvantage: Sensitive to outliers.

⑥ Recursive Least Squares Estimate:

Updates the estimate as new data comes in, based on principle of least squares.

Advantage: Saves computational resources.

Disadvantage: Depends on initial estimate.